refactor: derive string searcher from string pattern (#12312)
This PR reverses the relationship between the `ForwardPattern` and
`ToForwardSearcher` classes.

Previously, it was possible to derive `ForwardPattern` (i.e.,
`dropPrefix?`) from `ToForwardSearcher` (i.e., get an iterator of
`SearchStep (s)`). Now, we give the default instance in the other
direction: it is now possible to derive `ToForwardSearcher` from
`ForwardPattern`. Since it is usually much easier to provide
`ForwardPattern` than `ToForwardSearcher`, this means more shared code,
which pays off double since we will give a correctness proof for the
default implementation in an upcoming PR.

This PR also adds some string lemmas.

src/Init/Data/String/Pattern/Basic.lean
@@ -1,7 +1,7 @@
 /-
 Copyright (c) 2025 Lean FRO, LLC. All rights reserved.
 Released under Apache 2.0 license as described in the file LICENSE.
-Authors: Henrik Böving
+Authors: Henrik Böving, Markus Himmel
 -/
 module
 
@@ -9,6 +9,10 @@ prelude
 public import Init.Data.String.Basic
 public import Init.Data.Iterators.Basic
 public import Init.Data.Iterators.Consumers.Loop
+import Init.Data.String.Lemmas.IsEmpty
+import Init.Data.String.Termination
+import Init.Data.String.OrderInstances
+import Init.Data.String.Lemmas.Order
 
 set_option doc.verso true
 
@@ -41,9 +45,118 @@ inductive SearchStep (s : Slice) where
   | matched (startPos endPos : s.Pos)
 deriving Inhabited, BEq
 
+namespace SearchStep
+
+/-- The start position of a {name}`SearchStep`. -/
+@[inline]
+def startPos {s : Slice} (st : SearchStep s) : s.Pos :=
+  match st with
+  | .rejected startPos _ => startPos
+  | .matched startPos _ => startPos
+
+@[simp]
+theorem startPos_rejected {s : Slice} {p q : s.Pos} : (SearchStep.rejected p q).startPos = p := (rfl)
+
+@[simp]
+theorem startPos_matched {s : Slice} {p q : s.Pos} : (SearchStep.matched p q).startPos = p := (rfl)
+
+/-- The end position of a {name}`SearchStep`. -/
+@[inline]
+def endPos {s : Slice} (st : SearchStep s) : s.Pos :=
+  match st with
+  | .rejected _ endPos => endPos
+  | .matched _ endPos => endPos
+
+@[simp]
+theorem endPos_rejected {s : Slice} {p q : s.Pos} : (SearchStep.rejected p q).endPos = q := (rfl)
+
+@[simp]
+theorem endPos_matched {s : Slice} {p q : s.Pos} : (SearchStep.matched p q).endPos = q := (rfl)
+
+/--
+Converts a {lean}`SearchStep (s.sliceFrom p)` into a {lean}`SearchStep s` by applying
+{name}`Slice.Pos.ofSliceFrom` to the start and end position.
+-/
+def ofSliceFrom {s : Slice} {p : s.Pos} (st : SearchStep (s.sliceFrom p)) : SearchStep s :=
+  match st with
+  | .rejected l r => .rejected (Slice.Pos.ofSliceFrom l) (Slice.Pos.ofSliceFrom r)
+  | .matched l r => .matched (Slice.Pos.ofSliceFrom l) (Slice.Pos.ofSliceFrom r)
+
+@[simp]
+theorem startPos_ofSliceFrom {s : Slice} {p : s.Pos} {st : SearchStep (s.sliceFrom p)} :
+    st.ofSliceFrom.startPos = Slice.Pos.ofSliceFrom st.startPos := by
+  cases st <;>  simp [ofSliceFrom]
+
+@[simp]
+theorem endPos_ofSliceFrom {s : Slice} {p : s.Pos} {st : SearchStep (s.sliceFrom p)} :
+    st.ofSliceFrom.endPos = Slice.Pos.ofSliceFrom st.endPos := by
+  cases st <;> simp [ofSliceFrom]
+
+end SearchStep
+
+/--
+Provides simple pattern matching capabilities from the start of a {name}`Slice`.
+-/
+class ForwardPattern {ρ : Type} (pat : ρ) where
+  /--
+  Checks whether the slice starts with the pattern. If it does, the slice is returned with the
+  prefix removed; otherwise the result is {name}`none`.
+  -/
+  dropPrefix? : (s : Slice) →  Option s.Pos
+  /--
+  Checks whether the slice starts with the pattern. If it does, the slice is returned with the
+  prefix removed; otherwise the result is {name}`none`.
+  -/
+  dropPrefixOfNonempty? : (s : Slice) → (h : s.isEmpty = false) → Option s.Pos := fun s _ => dropPrefix? s
+  /--
+  Checks whether the slice starts with the pattern.
+  -/
+  startsWith : (s : Slice) → Bool := fun s => (dropPrefix? s).isSome
+
+/--
+A lawful forward pattern is one where the three functions {name}`ForwardPattern.dropPrefix?`,
+{name}`ForwardPattern.dropPrefixOfNonempty?` and {name}`ForwardPattern.startsWith` agree for any
+given input slice.
+
+Note that this is a relatively weak condition. It is non-uniform in the sense that the functions
+can still return completely different results on different slices, even if they represent the same
+string.
+
+There is a stronger lawfulness typeclass {lit}`LawfulForwardPatternModel` that asserts that the
+{name}`ForwardPattern.dropPrefix?` function behaves like a function that drops the longest prefix
+according to some notion of matching.
+-/
+class LawfulForwardPattern {ρ : Type} (pat : ρ) [ForwardPattern pat] : Prop where
+  dropPrefixOfNonempty?_eq {s : Slice} (h) :
+    ForwardPattern.dropPrefixOfNonempty? pat s h = ForwardPattern.dropPrefix? pat s
+  startsWith_eq (s : Slice) :
+    ForwardPattern.startsWith pat s = (ForwardPattern.dropPrefix? pat s).isSome
+
+/--
+A strict forward pattern is one which never drops an empty prefix.
+
+This condition ensures that the default searcher derived from the forward pattern is a finite
+iterator.
+-/
+class StrictForwardPattern {ρ : Type} (pat : ρ) [ForwardPattern pat] : Prop where
+  ne_startPos {s : Slice} (h) (q) :
+    ForwardPattern.dropPrefixOfNonempty? pat s h = some q → q ≠ s.startPos
+
 /--
 Provides a conversion from a pattern to an iterator of {name}`SearchStep` that searches for matches
 of the pattern from the start towards the end of a {name}`Slice`.
+
+While these operations can be implemented on top of {name}`ForwardPattern`, some patterns allow
+for more efficient implementations. For example, a searcher for {name}`String` patterns derived
+from the {name}`ForwardPattern` instance on strings would try to match the pattern at every
+position in the string, but more efficient string matching routines are known. Indeed, the Lean
+standard library uses the Knuth-Morris-Pratt algorithm. See the module
+{module -checked}`Init.Data.String.Pattern.String` for the implementation.
+
+This class can be used to provide such an efficient implementation. If there is no
+need to specialize in this fashion, then
+{name (scope := "Init.Data.String.Pattern.Basic")}`ToForwardSearcher.defaultImplementation` can be
+used to automatically derive an instance.
 -/
 class ToForwardSearcher {ρ : Type} (pat : ρ) (σ : outParam (Slice → Type)) where
   /--
@@ -53,25 +166,87 @@ class ToForwardSearcher {ρ : Type} (pat : ρ) (σ : outParam (Slice → Type)) 
   -/
   toSearcher : (s : Slice) → Std.Iter (α := σ s) (SearchStep s)
 
-/--
-Provides simple pattern matching capabilities from the start of a {name}`Slice`.
+namespace ToForwardSearcher
 
-While these operations can be implemented on top of {name}`ToForwardSearcher` some patterns allow
-for more efficient implementations. This class can be used to specialize for them. If there is no
-need to specialize in this fashion, then
-{name (scope := "Init.Data.String.Pattern.Basic")}`ForwardPattern.defaultImplementation` can be used
-to automatically derive an instance.
+structure DefaultForwardSearcher {ρ : Type} (pat : ρ) (s : Slice) where
+  currPos : s.Pos
+deriving Inhabited
+
+namespace DefaultForwardSearcher
+
+variable {ρ : Type} (pat : ρ)
+
+@[inline]
+def iter (s : Slice) : Std.Iter (α := DefaultForwardSearcher pat s) (SearchStep s) :=
+  ⟨⟨s.startPos⟩⟩
+
+instance (s : Slice) [ForwardPattern pat] :
+    Std.Iterator (DefaultForwardSearcher pat s) Id (SearchStep s) where
+  IsPlausibleStep it
+    | .yield it' (.rejected p₁ p₂) => ∃ (h : it.internalState.currPos ≠ s.endPos),
+      ForwardPattern.dropPrefixOfNonempty? pat (s.sliceFrom it.internalState.currPos) (by simpa) = none ∧
+      p₁ = it.internalState.currPos ∧ p₂ = it.internalState.currPos.next h ∧
+      it'.internalState.currPos = it.internalState.currPos.next h
+    | .yield it' (.matched p₁ p₂) => ∃ (h : it.internalState.currPos ≠ s.endPos), ∃ pos,
+      ForwardPattern.dropPrefixOfNonempty? pat (s.sliceFrom it.internalState.currPos) (by simpa) = some pos ∧
+      p₁ = it.internalState.currPos ∧ p₂ = Slice.Pos.ofSliceFrom pos ∧
+      it'.internalState.currPos = Slice.Pos.ofSliceFrom pos
+    | .done => it.internalState.currPos = s.endPos
+    | .skip _ => False
+  step it :=
+    if h : it.internalState.currPos = s.endPos then
+      pure (.deflate ⟨.done, by simp [h]⟩)
+    else
+      match h' : ForwardPattern.dropPrefixOfNonempty? pat (s.sliceFrom it.internalState.currPos) (by simpa) with
+      | some pos =>
+        pure (.deflate ⟨.yield ⟨⟨Slice.Pos.ofSliceFrom pos⟩⟩
+          (.matched it.internalState.currPos (Slice.Pos.ofSliceFrom pos)), by simp [h, h']⟩)
+      | none =>
+        pure (.deflate ⟨.yield ⟨⟨it.internalState.currPos.next h⟩⟩
+          (.rejected it.internalState.currPos (it.internalState.currPos.next h)), by simp [h, h']⟩)
+
+private def finitenessRelation (s : Slice) [ForwardPattern pat] [StrictForwardPattern pat] :
+    Std.Iterators.FinitenessRelation (DefaultForwardSearcher pat s) Id where
+  Rel := InvImage WellFoundedRelation.rel (fun it => it.internalState.currPos)
+  wf := InvImage.wf _ WellFoundedRelation.wf
+  subrelation {it it'} h := by
+    simp_wf
+    obtain ⟨step, h, h'⟩ := h
+    match step with
+    | .yield it'' (.rejected p₁ p₂) =>
+      obtain ⟨_, ⟨-, -, -, h'⟩⟩ := h'
+      cases h
+      simp [h']
+    | .yield it'' (.matched p₁ p₂) =>
+      obtain ⟨_, pos, ⟨h₀, -, -, h'⟩⟩ := h'
+      cases h
+      have := StrictForwardPattern.ne_startPos _ _ h₀
+      rw [h']
+      exact Std.lt_of_le_of_lt Slice.Pos.le_ofSliceFrom
+        (Slice.Pos.ofSliceFrom_lt_ofSliceFrom_iff.2 ((Slice.Pos.startPos_lt_iff _).2 this))
+
+instance {s : Slice} [ForwardPattern pat] [StrictForwardPattern pat] :
+    Std.Iterators.Finite (DefaultForwardSearcher pat s) Id :=
+  .of_finitenessRelation (finitenessRelation pat s)
+
+instance [ForwardPattern pat] : Std.IteratorLoop (DefaultForwardSearcher pat s) Id Id :=
+  .defaultImplementation
+
+end DefaultForwardSearcher
+
+/--
+The default implementation of {name}`ToForwardSearcher` repeatedly tries to match the pattern using
+the given {name}`ForwardPattern` instance.
+
+It is sometimes possible to give a more efficient implementation; see {name}`ToForwardSearcher`
+for more details.
 -/
-class ForwardPattern {ρ : Type} (pat : ρ) where
-  /--
-  Checks whether the slice starts with the pattern.
-  -/
-  startsWith : Slice → Bool
-  /--
-  Checks whether the slice starts with the pattern. If it does, the slice is returned with the
-  prefix removed; otherwise the result is {name}`none`.
-  -/
-  dropPrefix? : (s : Slice) → Option s.Pos
+@[inline]
+def defaultImplementation [ForwardPattern pat] :
+    ToForwardSearcher pat (DefaultForwardSearcher pat) where
+  toSearcher := DefaultForwardSearcher.iter pat
+
+end ToForwardSearcher
 
 namespace Internal
 
@@ -123,37 +298,69 @@ def memcmpSlice (lhs rhs : Slice) (lstart : String.Pos.Raw) (rstart : String.Pos
 
 end Internal
 
-namespace ForwardPattern
+/--
+Provides simple pattern matching capabilities from the end of a {name}`Slice`.
+-/
+class BackwardPattern {ρ : Type} (pat : ρ) where
+  /--
+  Checks whether the slice ends with the pattern. If it does, the slice is returned with the
+  suffix removed; otherwise the result is {name}`none`.
+  -/
+  dropSuffix? : (s : Slice) → Option s.Pos
+  /--
+  Checks whether the slice ends with the pattern. If it does, the slice is returned with the
+  suffix removed; otherwise the result is {name}`none`.
+  -/
+  dropSuffixOfNonempty? : (s : Slice) → (h : s.isEmpty = false) → Option s.Pos := fun s _ => dropSuffix? s
+  /--
+  Checks whether the slice ends with the pattern.
+  -/
+  endsWith : Slice → Bool := fun s => (dropSuffix? s).isSome
 
-variable {ρ : Type} {σ : Slice → Type}
-variable [∀ s, Std.Iterator (σ s) Id (SearchStep s)]
-variable (pat : ρ) [ToForwardSearcher pat σ]
+/--
+A lawful backward pattern is one where the three functions {name}`BackwardPattern.dropSuffix?`,
+{name}`BackwardPattern.dropSuffixOfNonempty?` and {name}`BackwardPattern.endsWith` agree for any
+given input slice.
 
-@[specialize pat]
-def defaultStartsWith (s : Slice) [Std.IteratorLoop (σ s) Id Id] : Bool :=
-  let searcher := ToForwardSearcher.toSearcher pat s
-  match searcher.first? with
-  | some (.matched start ..) => s.startPos = start
-  | _ => false
+Note that this is a relatively weak condition. It is non-uniform in the sense that the functions
+can still return completely different results on different slices, even if they represent the same
+string.
 
-@[specialize pat]
-def defaultDropPrefix? (s : Slice) [Std.IteratorLoop (σ s) Id Id] : Option s.Pos :=
-  let searcher := ToForwardSearcher.toSearcher pat s
-  match searcher.first? with
-  | some (.matched _ endPos) => some endPos
-  | _ => none
+There is a stronger lawfulness typeclass {lit}`LawfulBackwardPatternModel` that asserts that the
+{name}`BackwardPattern.dropSuffix?` function behaves like a function that drops the longest prefix
+according to some notion of matching.
+-/
+class LawfulBackwardPattern {ρ : Type} (pat : ρ) [BackwardPattern pat] : Prop where
+  dropSuffixOfNonempty?_eq {s : Slice} (h) :
+    BackwardPattern.dropSuffixOfNonempty? pat s h = BackwardPattern.dropSuffix? pat s
+  endsWith_eq (s : Slice) :
+    BackwardPattern.endsWith pat s = (BackwardPattern.dropSuffix? pat s).isSome
 
-@[always_inline, inline]
-def defaultImplementation {pat : ρ} [ToForwardSearcher pat σ] [∀ s, Std.IteratorLoop (σ s) Id Id] :
-    ForwardPattern pat where
-  startsWith s := defaultStartsWith pat s
-  dropPrefix? s := defaultDropPrefix? pat s
+/--
+A strict backward pattern is one which never drops an empty suffix.
 
-end ForwardPattern
+This condition ensures that the default searcher derived from the backward pattern is a finite
+iterator.
+-/
+class StrictBackwardPattern {ρ : Type} (pat : ρ) [BackwardPattern pat] : Prop where
+  ne_endPos {s : Slice} (h) (q) :
+    BackwardPattern.dropSuffixOfNonempty? pat s h = some q → q ≠ s.endPos
 
 /--
 Provides a conversion from a pattern to an iterator of {name}`SearchStep` searching for matches of
 the pattern from the end towards the start of a {name}`Slice`.
+
+While these operations can be implemented on top of {name}`BackwardPattern`, some patterns allow
+for more efficient implementations. For example, a searcher for {name}`String` patterns derived
+from the {name}`BackwardPattern` instance on strings would try to match the pattern at every
+position in the string, but more efficient string matching routines are known. Indeed, the Lean
+standard library uses the Knuth-Morris-Pratt algorithm. See the module
+{module -checked}`Init.Data.String.Pattern.String` for the implementation.
+
+This class can be used to provide such an efficient implementation. If there is no
+need to specialize in this fashion, then
+{name (scope := "Init.Data.String.Pattern.Basic")}`ToBackwardSearcher.defaultImplementation` can be
+used to automatically derive an instance.
 -/
 class ToBackwardSearcher {ρ : Type} (pat : ρ) (σ : outParam (Slice → Type)) where
   /--
@@ -163,51 +370,84 @@ class ToBackwardSearcher {ρ : Type} (pat : ρ) (σ : outParam (Slice → Type))
   -/
   toSearcher : (s : Slice) → Std.Iter (α := σ s) (SearchStep s)
 
-/--
-Provides simple pattern matching capabilities from the end of a {name}`Slice`.
-
-While these operations can be implemented on top of {name}`ToBackwardSearcher`, some patterns allow
-for more efficient implementations. This class can be used to specialize for them. If there is no
-need to specialize in this fashion, then
-{name (scope := "Init.Data.String.Pattern.Basic")}`BackwardPattern.defaultImplementation` can be
-used to automatically derive an instance.
--/
-class BackwardPattern {ρ : Type} (pat : ρ) where
-  /--
-  Checks whether the slice ends with the pattern.
-  -/
-  endsWith : Slice → Bool
-  /--
-  Checks whether the slice ends with the pattern. If it does, the slice is returned with the
-  suffix removed; otherwise the result is {name}`none`.
-  -/
-  dropSuffix? : (s : Slice) → Option s.Pos
-
 namespace ToBackwardSearcher
 
-variable {ρ : Type} {σ : Slice → Type}
-variable [∀ s, Std.Iterator (σ s) Id (SearchStep s)]
-variable (pat : ρ) [ToBackwardSearcher pat σ]
+structure DefaultBackwardSearcher {ρ : Type} (pat : ρ) (s : Slice) where
+  currPos : s.Pos
+deriving Inhabited
 
-@[specialize pat]
-def defaultEndsWith (s : Slice) [Std.IteratorLoop (σ s) Id Id] : Bool :=
-  let searcher := ToBackwardSearcher.toSearcher pat s
-  match searcher.first? with
-  | some (.matched _ endPos) => s.endPos = endPos
-  | _ => false
+namespace DefaultBackwardSearcher
 
-@[specialize pat]
-def defaultDropSuffix? (s : Slice) [Std.IteratorLoop (σ s) Id Id] : Option s.Pos :=
-  let searcher := ToBackwardSearcher.toSearcher pat s
-  match searcher.first? with
-  | some (.matched startPos _) => some startPos
-  | _ => none
+variable {ρ : Type} (pat : ρ)
 
-@[always_inline, inline]
-def defaultImplementation {pat : ρ} [ToBackwardSearcher pat σ] [∀ s, Std.IteratorLoop (σ s) Id Id] :
-    BackwardPattern pat where
-  endsWith s := defaultEndsWith pat s
-  dropSuffix? s := defaultDropSuffix? pat s
+@[inline]
+def iter (s : Slice) : Std.Iter (α := DefaultBackwardSearcher pat s) (SearchStep s) :=
+  ⟨⟨s.endPos⟩⟩
+
+instance (s : Slice) [BackwardPattern pat] :
+    Std.Iterator (DefaultBackwardSearcher pat s) Id (SearchStep s) where
+  IsPlausibleStep it
+    | .yield it' (.rejected p₁ p₂) => ∃ (h : it.internalState.currPos ≠ s.startPos),
+      BackwardPattern.dropSuffixOfNonempty? pat (s.sliceTo it.internalState.currPos) (by simpa) = none ∧
+      p₁ = it.internalState.currPos.prev h ∧ p₂ = it.internalState.currPos  ∧
+      it'.internalState.currPos = it.internalState.currPos.prev h
+    | .yield it' (.matched p₁ p₂) => ∃ (h : it.internalState.currPos ≠ s.startPos), ∃ pos,
+      BackwardPattern.dropSuffixOfNonempty? pat (s.sliceTo it.internalState.currPos) (by simpa) = some pos ∧
+      p₁ = Slice.Pos.ofSliceTo pos ∧ p₂ = it.internalState.currPos  ∧
+      it'.internalState.currPos = Slice.Pos.ofSliceTo pos
+    | .done => it.internalState.currPos = s.startPos
+    | .skip _ => False
+  step it :=
+    if h : it.internalState.currPos = s.startPos then
+      pure (.deflate ⟨.done, by simp [h]⟩)
+    else
+      match h' : BackwardPattern.dropSuffixOfNonempty? pat (s.sliceTo it.internalState.currPos) (by simpa) with
+      | some pos =>
+        pure (.deflate ⟨.yield ⟨⟨Slice.Pos.ofSliceTo pos⟩⟩
+          (.matched (Slice.Pos.ofSliceTo pos) it.internalState.currPos), by simp [h, h']⟩)
+      | none =>
+        pure (.deflate ⟨.yield ⟨⟨it.internalState.currPos.prev h⟩⟩
+          (.rejected (it.internalState.currPos.prev h) it.internalState.currPos), by simp [h, h']⟩)
+
+private def finitenessRelation (s : Slice) [BackwardPattern pat] [StrictBackwardPattern pat] :
+    Std.Iterators.FinitenessRelation (DefaultBackwardSearcher pat s) Id where
+  Rel := InvImage WellFoundedRelation.rel (fun it => it.internalState.currPos.down)
+  wf := InvImage.wf _ WellFoundedRelation.wf
+  subrelation {it it'} h := by
+    simp_wf
+    obtain ⟨step, h, h'⟩ := h
+    match step with
+    | .yield it'' (.rejected p₁ p₂) =>
+      obtain ⟨_, ⟨-, -, -, h'⟩⟩ := h'
+      cases h
+      simp [h']
+    | .yield it'' (.matched p₁ p₂) =>
+      obtain ⟨_, pos, ⟨h₀, -, -, h'⟩⟩ := h'
+      cases h
+      have := StrictBackwardPattern.ne_endPos _ _ h₀
+      rw [h']
+      exact Std.lt_of_lt_of_le (Slice.Pos.ofSliceTo_lt_ofSliceTo_iff.2 ((Slice.Pos.lt_endPos_iff _).2 this)) Slice.Pos.ofSliceTo_le
+
+instance {s : Slice} [BackwardPattern pat] [StrictBackwardPattern pat] :
+    Std.Iterators.Finite (DefaultBackwardSearcher pat s) Id :=
+  .of_finitenessRelation (finitenessRelation pat s)
+
+instance [BackwardPattern pat] : Std.IteratorLoop (DefaultBackwardSearcher pat s) Id Id :=
+  .defaultImplementation
+
+end DefaultBackwardSearcher
+
+/--
+The default implementation of {name}`ToBackwardSearcher` repeatedly tries to match the pattern using
+the given {name}`BackwardPattern` instance.
+
+It is sometimes possible to give a more efficient implementation; see {name}`ToBackwardSearcher`
+for more details.
+-/
+@[inline]
+def defaultImplementation [BackwardPattern pat] :
+    ToBackwardSearcher pat (DefaultBackwardSearcher pat) where
+  toSearcher := DefaultBackwardSearcher.iter pat
 
 end ToBackwardSearcher
 
